\documentclass[10pt, a4paper]{article}

%%%%%%%%%%%%%%
%  Packages  %
%%%%%%%%%%%%%%


\usepackage{page_format}
\usepackage{special}
\usepackage{hyperref}
\usepackage{tikz}
\usepackage[compat=1.1.0]{tikz-feynman}
\input{math_func}

\usepackage{slashed}

% References
\usepackage{biblatex}
\addbibresource{ref.bib}
\usetikzlibrary{positioning}


%%%%%%%%%%%%
%  Colors  %
%%%%%%%%%%%%
% ! EDIT HERE !
\colorlet{chaptercolor}{red!70!black} % Foreground color.
\colorlet{chaptercolorback}{red!10!white} % Background color

%%%%%%%%%%%%%%
% Page titre %
%%%%%%%%%%%%%%%
\title{Homework 1} % Title of the assignement.
\author{\PA} % Your name(s).
\teacher{Jaume Gomis and Mykola Semenyakin} % Your teacher's name.
\class{Quantum Field Theory III} % The class title.

\university{Perimeter Institute for Theoretical Physics} % University
\faculty{Perimeter Scholars International} % Faculty
%\departement{<Departement>} % Departement
\date{\today} % Date.


%%%%%%%%%%%%%%%%%%%%%%
% Begin the document %
%%%%%%%%%%%%%%%%%%%%%%
\begin{document}

% Make the title page.
\maketitlepage

% Make table of contents
\maketableofcontents

% Assignment starts here ----------------------------

\footnotesize{

\section{Conformal invariance of the Maxwell action for $D=4$}

\begin{enumerate}
  \item[(a)] Consider a classical abelian gauge field $A_\mu$ on $D=4$ dimensionnal Minkowski spacetime. Under an infinitesimal conformal transformation, spacetime undergoes the transformation $\tilde{x}^{\mu} = f(x) = x^{\mu} + \xi^{\mu}(x)$ where $\xi^\mu(x)$ is a smal deformation. We want to calculate the effect of this transformation on the gauge field $A_\mu$. The starting point is that we expect $A_\mu$ to transform as a tensor under the lorenz transformation subgroup of the conformal group. This implies that $A_\mu$ is a primary operator and we denote its scaling dimension $\Delta$. The transformed field $\tilde{A}_\mu$ at $\tilde{x}$ is related to the original field $A_\mu$ at $x$ by an internal rotation, scaling, and special conformal transformation. The rotation operation acts on the components $A_\mu$ through its spin $1$ representation which is the defnining representation of rotations. The scaling and special conformal transformation act together through the multiplication of $A_\mu$ by the jacobian factor $|\partial x/\partial \tilde{x}|_{x}^{\Delta/D}$. Finally, translations act trivially internally. This can be summarized with the relation $\tilde{A}_\mu(\tilde x) = |\partial x/\partial \tilde{x}|_{x}^{\Delta/D} R_{\mu}^{\nu} A_{\nu}(x)$ where $R_{\mu}^{\nu}$ is the matrix associated with the part of $\xi^\mu(x)$ that does not change the metric components (after the Weyl and diffeomorpshim transformations). With this in mind, we calculate the jacobian of the infinitesimal transformation to be 
  \begin{align*}
    \left|\frac{\partial x^\mu }{\partial \tilde{x}^\nu}\right|_{x} = \left|\frac{\partial \tilde{x}^\mu }{\partial x^\nu}\right|_{x}^{-1} = |\delta_\nu^\mu + \partial_\nu \xi^\mu|_{x}^{-1} \approx |e^{-\partial_\nu \xi^\mu}|_{x} = e^{-\text{Tr} \partial_\nu \xi^\mu(x)} = 1- \partial_\mu \xi^\mu(x) + O(\xi^2). 
  \end{align*}
  The matrix $R_{\mu}^{\nu} (x)$ can be extracted by dividing the matrix $(\partial x/\partial \tilde{x})_{x}$ by a factor $\Omega(x)$ such that we extract the "metric component preserving" operation. To find this factor we consider the effect on the metric of $\Omega^{-1}(x)(\partial x/\partial \tilde{x})_{x}$. We can write the "metric component preserving" property as
  \begin{align*}
    \Omega^{-2}(x) \left(\frac{\partial x^{\mu}}{\partial \tilde{x}^\sigma}\right)_{x} \left(\frac{\partial x^\nu}{\partial \tilde{x}^{\rho}}\right)_{x} \eta_{\mu\nu} = \eta_{\sigma \rho}.
  \end{align*}
  Since $\Omega(x)$ is a factor, we can extract it by taking the determinant on both sides of the previous relation to get 
  \begin{align*}
    \det(\eta) \Omega(x)^{-2D} \left|\frac{\partial x^\mu }{\partial \tilde{x}^\nu}\right|_{x}^2 = \det(\eta) \iff \Omega(x) = \left|\frac{\partial x^\mu }{\partial \tilde{x}^\nu}\right|_{x}^{-\frac{1}{D}}.
  \end{align*}
  This result can be intuitively undertsood from the fact the jacobian measures $D$-volume rescaling. Since we want metric components (associated to distances) to be preserved by the rescaled trasnformation, we need to divide by the $D$-root of the jacobian. The matrix $R_{\mu}^{\nu} (x)$ provided by the rescaling is given by 
  \begin{align*}
    R_{\mu}^{\nu} (x) = \frac{1}{(1- \partial_\sigma \xi^\sigma(x) + O(\xi^2))^{1/D}} \left(\frac{\partial x^\nu }{\partial \tilde{x}^\mu}\right)_{x} &= (1 + \partial_\sigma \xi^\sigma(x)/D + O(\xi^2))(\delta_\nu^\mu + \partial_\mu \xi^\nu(x) + O(\xi^2))^{-1}\\
    &= \delta_\nu^\mu(1 + \partial_\sigma \xi^\sigma(x)/D)  - \partial_\mu \xi^\nu(x) +  O(\xi^2). 
  \end{align*} 
  We note that $R_{\mu}^{\nu} (x)$ will represent a rotation if $\partial_\sigma \xi^\sigma(x) = 0$ (bring the conformal Killing equation to the normal Killing equation with a rotation isometry as its solution). If $\partial_\sigma \xi^\sigma(x) \neq 0$, the rescaled transformation contains a special conformal trasformation. The special conformal transformation as a Weyl transformation does not preserve distances, but can be combined with a diffeomorpshim to preserve the initial components of the metric. With these results, we can write the effect of the infinitesimal transformation as 
  \begin{align*}
    \tilde{A}_\mu(\tilde{x}) &= (1-\partial_\rho \xi^\rho(f^{-1}(\tilde{x})) + O(\xi^2))^{\Delta/D} (A_\mu(f^{-1}(\tilde{x})) + A_\mu(f^{-1}(\tilde{x})) \partial_\sigma \xi^\sigma(f^{-1}(\tilde{x}))\frac{1}{D}  - A_\nu(f^{-1}(\tilde{x})) \partial_\mu \xi^\nu(f^{-1}(\tilde{x})) +  O(\xi^2)) \\
    &=  \left(1-\frac{\Delta}{D}\partial_\rho \xi^\rho(f^{-1}(\tilde{x})) + O(\xi^2)\right) (A_\mu(f^{-1}(\tilde{x})) + A_\mu(f^{-1}(\tilde{x})) \partial_\sigma \xi^\sigma(f^{-1}(\tilde{x}))\frac{1}{D} - A_\nu(f^{-1}(\tilde{x})) \partial_\mu \xi^\nu(f^{-1}(\tilde{x})) +  O(\xi^2))\\
    &= A_\mu(f^{-1}(\tilde{x}))-A_\mu(f^{-1}(\tilde{x})) \frac{\Delta}{D}\partial_\sigma \xi^\sigma(f^{-1}(\tilde{x}))+A_\mu(f^{-1}(\tilde{x})) \partial_\sigma \xi^\sigma(f^{-1}(\tilde{x})) \frac{1}{D}  - A_\nu(f^{-1}(\tilde{x})) \partial_\mu \xi^\nu(f^{-1}(\tilde{x})) + O(\xi^2). 
  \end{align*}
  Since $\xi(f^{-1}(\tilde{x}))$ is already first order in $\xi$, the only term contribution to its expansion around $\xi = 0$ at $O(\xi)$ is $\xi(\tilde{x})$. To go further, we expand $f^{-1}(\tilde{x})$ at first order in $\xi(\tilde{x})$ with the ansatz $f^{-1}(\tilde{x})^{\nu} = \tilde{x}^{\nu} + B_{\mu}^{\nu}(\tilde{x}) \xi^{\mu}(\tilde{x})$ (the first term of this ansatz is justified by noticing the transformation reduces to identity at $\xi = 0$).  From $f(f^{-1}(\tilde{x})) = \tilde{x}$, we find 
  \begin{align*}
    \tilde{x}^{\nu} = \tilde{x}^{\nu} + B_\mu^{\nu}(\tilde{x}) \xi^\mu(\tilde{x}) + \xi(\tilde{x}^{\nu} +  B_\mu^{\nu}(\tilde{x}) \xi^\mu(\tilde{x})) + O(\xi^2) \implies B_\mu^{\nu}(\tilde{x}) \xi^\mu(\tilde{x}) + \xi^{\nu}(\tilde{x}) = 0, \quad  \forall \xi(\tilde{x}) \implies B_\mu^{\nu}(\tilde{x}) = -\delta_{\mu}^{\nu}.
  \end{align*}
  Using this result, we can expand $A_\mu(f^{-1}(\tilde{x}))$ as 
  \begin{align*}
    A_\mu(f^{-1}(\tilde{x})) = A_\mu(\tilde{x}^\nu-\xi^{\nu}(\tilde{x}) + O(\xi^2)) = A_\mu(\tilde{x}) - \xi^{\nu}(\tilde{x}) \partial_\nu A_\mu(\tilde{x}) + O(\xi^2)
  \end{align*}
  Combining this expression with the internal transformation at first order in $\xi$, we get 
  \begin{align*}
    \tilde{A}_\mu(\tilde{x}) &= \left(1-\frac{\Delta}{D}\partial_\sigma \xi^\sigma(\tilde{x})+\partial_\sigma \xi^\sigma(\tilde{x})  - \partial_\mu \xi^\nu(\tilde{x})\right)(A_\mu(\tilde{x}) - \xi^{\nu}(\tilde{x}) \partial_\nu A_\mu(\tilde{x})) + O(\xi^2)\\
    &= A_\mu(\tilde{x})-A_\mu(\tilde{x}) \frac{\Delta-1}{D}\partial_\sigma \xi^\sigma(\tilde{x}) - A_\nu(\tilde{x})\partial_\mu \xi^\nu(\tilde{x}) - \xi^{\nu}(\tilde{x}) \partial_\nu A_\mu(\tilde{x})+ O(\xi^2)
  \end{align*}
  with $\xi(f^{-1}(\tilde{x})) = \xi(\tilde{x}) + O(\xi^2)$. This result can be simplified by using the conformal killing equation $\partial_\mu \xi_\nu+\partial_\nu \xi_\mu=2 \eta_{\mu \nu} \partial_\sigma  \xi^\sigma/D$ as follows:
  \begin{align*}
    \tilde{A}_\mu(\tilde{x}) &= A_\mu(\tilde{x})-A_\mu(\tilde{x}) \frac{\Delta-1}{D}\partial_\sigma \xi^\sigma(\tilde{x}) - A_\nu(\tilde{x})\left(\frac{1}{2}\partial_\mu \xi^\nu(\tilde{x}) + \frac{1}{2}\partial_\mu \xi^\nu(\tilde{x})\right) - \xi^{\nu}(\tilde{x}) \partial_\nu A_\mu(\tilde{x})+ O(\xi^2)\\
    &= A_\mu(\tilde{x})-A_\mu(\tilde{x}) \frac{\Delta-1}{D}\partial_\sigma \xi^\sigma(\tilde{x}) - A_\nu(\tilde{x})\left(\frac{1}{2}\partial_\mu \xi^\nu(\tilde{x}) - \frac{1}{2}\partial_\nu \xi^\mu(\tilde{x}) + \delta_{\mu}^{\nu} \partial_\sigma \xi^\sigma(\tilde{x}) \frac{1}{D}\right) - \xi^{\nu}(\tilde{x}) \partial_\nu A_\mu(\tilde{x})+ O(\xi^2)\\
    &= A_\mu(\tilde{x})-A_\mu(\tilde{x}) \frac{\Delta}{D}\partial_\sigma \xi^\sigma(\tilde{x}) - A_\nu(\tilde{x})\underbrace{\left(\frac{1}{2}\partial_\mu \xi^\nu(\tilde{x}) - \frac{1}{2}\partial^\nu \xi_\mu(\tilde{x})\right)}_{M_{\mu}{}^{\nu}} - \xi^{\nu}(\tilde{x}) \partial_\nu A_\mu(\tilde{x})+ O(\xi^2).
  \end{align*}
  From this transformed gauge field, we calculate the transformation of gauge field strength $F_{\mu\nu} = \partial_\mu A_\nu - \partial_\nu A_\mu$ to $\tilde{F}_{\mu\nu}$. We start by writting the transformation law of the derivatives used to construct $F_{\mu\nu}$. The chain rule yields
  \begin{align*}
    \tilde{\partial}_{\mu} \equiv \frac{\partial }{\partial \tilde{x}^\mu} = \left(\frac{\partial f^{-1}(\tilde{x})^\nu}{\partial \tilde{x}^\mu}\right)_{\tilde{x}}\left(\frac{\partial }{\partial x^\nu}\right)_{\tilde{x}} = \left(\frac{\partial \tilde{x}^{\nu} - \xi^{\nu}(\tilde{x})}{\partial \tilde{x}^\mu}\right)_{\tilde{x}}\left(\frac{\partial }{\partial x^\nu}\right)_{\tilde{x}} = \left(-\frac{\partial \xi^{\nu}(\tilde{x})}{\partial \tilde{x}^\mu}\right)_{\tilde{x}}\left(\frac{\partial }{\partial x^\nu}\right)_{\tilde{x}} + \left(\frac{\partial }{\partial x^\mu}\right)_{\tilde{x}} \equiv -\partial_\mu \xi^{\nu}(\tilde{x}) \partial_\nu + \partial_\mu. 
  \end{align*}
  where the subscripts indicate thet a partial derivative with respect to $x^\mu$ should be precomposed with $x = f^{-1}(x^{\mu})$ to yield a function dependant on the left hand side variable $\tilde{x}$. Now we can calculate the transformed field strength at first order in $\xi$ to be 
  \begin{align*}
    \tilde{F}_{\mu\nu} &= \tilde{\partial}_\mu \tilde{A}_{\nu} - (\mu \leftrightarrow \nu) \\
    &= \left(-\partial_\mu \xi^{\rho}(\tilde{x}) \partial_\rho + \partial_\mu\right)\left(A_\nu(\tilde{x})-A_\nu(\tilde{x}) \frac{\Delta}{D}\partial_\sigma \xi^\sigma(\tilde{x}) - A_\lambda(\tilde{x})M_{\nu}{}^{\lambda} - \xi^{\lambda}(\tilde{x}) \partial_\lambda A_\nu(\tilde{x})\right)- (\mu \leftrightarrow \nu)\\
    &= \partial_\mu A_\nu(\tilde{x}) - (\partial_\mu \xi^{\lambda}(\tilde{x})) \partial_\lambda A_\nu(\tilde{x}) -\partial_\mu \left(A_\nu(\tilde{x}) \frac{\Delta}{D}\partial_\lambda \xi^\lambda(\tilde{x})\right) - \partial_\mu\left(A_\lambda(\tilde{x})M_{\nu}{}^{\lambda}\right) - \partial_\mu\left(\xi^{\lambda}(\tilde{x}) \partial_\lambda A_\nu(\tilde{x})\right) - (\mu \leftrightarrow \nu)\\
    &= \partial_\mu A_\nu(\tilde{x}) -\partial_\mu \left(A_\nu(\tilde{x}) \frac{\Delta}{D}\partial_\lambda \xi^\lambda(\tilde{x})\right) - \partial_\mu A_\lambda(\tilde{x})\partial_\nu \xi^\lambda(\tilde{x}) - A_\lambda(\tilde{x})\partial_\mu\partial_\nu \xi^\lambda(\tilde{x}) - \xi^{\lambda}(\tilde{x}) \partial_\lambda \partial_\mu A_\nu(\tilde{x}) - 2(\partial_\mu \xi^{\lambda}(\tilde{x})) \partial_\lambda A_\nu(\tilde{x}) - (\mu \leftrightarrow \nu)\\
    &= \partial_\mu A_\nu(\tilde{x}) -\partial_\mu \left(A_\nu(\tilde{x}) \frac{\Delta}{D}\partial_\lambda \xi^\lambda(\tilde{x})\right) - (\partial_\mu A_\lambda(\tilde{x}))M_{\nu}{}^{\lambda} - A_\lambda(\tilde{x})\partial_\mu M_{\nu}{}^{\lambda} - \xi^{\lambda}(\tilde{x}) \partial_\lambda \partial_\mu A_\nu(\tilde{x}) - 2(\partial_\mu \xi^{\lambda}(\tilde{x})) \partial_\lambda A_\nu(\tilde{x}) - (\mu \leftrightarrow \nu)\\
    &= F_{\mu \nu}(\tilde{x}) - F_{\mu \nu}(\tilde{x}) \frac{\Delta}{D}\partial_\lambda \xi^\lambda(\tilde{x}) - A_{(\nu}(\tilde{x}) \frac{\Delta}{D}\partial_{\mu)} \partial_\lambda \xi^\lambda(\tilde{x})  - (\partial_{(\mu} A_\lambda(\tilde{x}))M_{\nu)}{}^{\lambda} - A_\lambda(\tilde{x})\partial_{(\mu} M_{\nu)}{}^{\lambda} - \xi^{\lambda}(\tilde{x}) \partial_\lambda F_{\mu\nu}(\tilde{x}) - 2(\partial_{(\mu} \xi^{\lambda}(\tilde{x})) \partial_\lambda A_{\nu)}(\tilde{x})\\
    &= F_{\mu \nu}(\tilde{x}) - F_{\mu \nu}(\tilde{x}) \frac{\Delta}{D}\partial_\lambda \xi^\lambda(\tilde{x}) - A_{(\nu}(\tilde{x}) \frac{\Delta}{D}\partial_{\mu)} \partial_\lambda \xi^\lambda(\tilde{x})  - (\partial_{(\mu} A_\lambda(\tilde{x}))M_{\nu)}{}^{\lambda} - \xi^{\lambda}(\tilde{x}) \partial_\lambda F_{\mu\nu}(\tilde{x}) - 2(\partial_{(\mu} \xi^{\lambda}(\tilde{x})) \partial_\lambda A_{\nu)}(\tilde{x})
  \end{align*}
  where we simplified further by expliciting 
  \begin{align*}
    & 2\partial_{(\mu} M_{\nu)}{}^{\lambda} = \partial_\mu\partial_\nu \xi^\lambda(\tilde{x}) - \partial_\mu\partial^\lambda \xi_\nu(\tilde{x}) - \partial_\nu \partial_\mu \xi^\lambda(\tilde{x}) - \partial_\nu \partial^\lambda \xi_\mu(\tilde{x}) = 0.
  \end{align*}
  We note that the transformation law of $F_{\mu\nu}$ involves $A_{\mu}$ homogeneously which is an example of mixing of CFT fields under the transformation of a descendant. 
  \item[(b)] For a $D$-dimensionnal spacetime, the Maxwell action reads 
  \begin{align*}
    S = \int \text{d}^D x \sqrt{|g|} \frac{1}{4} F_{\mu\nu} F^{\mu \nu} = \int \text{d}^D x \sqrt{|g|} \ g^{\mu \sigma} g^{\nu \rho}\frac{1}{4} F_{\mu\nu} F_{\sigma \rho}.  
  \end{align*}
  where $g$ is the metric (which we suppose conformaly flat). We aim to apply the results found in (a) to determine when this action gains conformal symmetry. Under a conformal transformation given by the killing vector $\xi^{\mu}(x)$ and the scaling $\Omega(x) = 1 + \partial_\mu \xi^\mu(x)/D + O(\xi^2)$ of the metric components, we have 
  \begin{align*}
    &g_{\nu \rho}(x) = \Omega(f(x))^{-2} \tilde{g}_{\nu \rho}(f(x)) = \Omega(\tilde{x})^{-2} \tilde{g}_{\nu \rho}(\tilde{x}) \quad \text{Defining property of a conformal transformation}\\
    &|g|(x) = \Omega(f(x))^{-2D} |\tilde{g}|(f(x)), \quad g^{\nu \rho}(x) = \Omega(f(x))^{+2} \tilde{g}^{\nu \rho}(f(x)) = \Omega(\tilde{x})^{2} \tilde{g}^{\nu \rho}(\tilde{x}), \quad  \text{d}^D x \sqrt{|g|} = \text{d}^D \tilde{x}\ \Omega(\tilde{x})^{-D} \sqrt{|\tilde{g}|(\tilde{x})}
  \end{align*}
  Without loss of generality, we take the traget metric $\tilde{g}$ to be the Minkowski metric.
  Inverting the result found in (a) for the transformation of the gauge field, we write 
  \begin{align*}
    A_{\mu}(x) =  |\partial x/\partial \tilde{x}|_{\tilde{x}}^{-\Delta/D} (R^{-1})_{\mu}^{\nu} \tilde{A}_{\nu}(\tilde{x}) &= \tilde{A}_\mu(\tilde{x})+\tilde{A}_\mu(\tilde{x}) \frac{\Delta}{D}\partial_\sigma \xi^\sigma(\tilde{x})-\tilde{A}_\mu(\tilde{x}) \partial_\sigma \xi^\sigma(\tilde{x}) \frac{1}{D}  + \tilde{A}_\nu(\tilde{x}) \partial_\mu \xi^\nu(\tilde{x}) + O(\xi^2) \\
    &= \tilde{A}_\mu(\tilde{x})+\tilde{A}_\mu(\tilde{x}) \frac{\Delta}{D}\partial_\sigma \xi^\sigma(\tilde{x}) + \frac{1}{2}\tilde{A}_\nu(\tilde{x}) \left(\partial_\mu \xi^\nu(\tilde{x}) - \partial^\nu \xi_\mu(\tilde{x})\right) + O(\xi^2). 
  \end{align*}
  Then, with the derivative $(\partial_{\mu})_{\tilde{x}} = \tilde{\partial}_\mu \xi^{\nu}(\tilde{x}) \tilde{\partial}_\nu + \tilde{\partial}_\mu$, the field strength transforms as 
  \begin{align*}
    F_{\mu \nu} = \partial_\mu A_{\nu}(x) - (\mu \leftrightarrow \nu) &= \left( \tilde{\partial}_\mu \xi^{\lambda}(\tilde{x}) \tilde{\partial}_\lambda + \tilde{\partial}_\mu\right)\left(\tilde{A}_\nu(\tilde{x})+\tilde{A}_\nu(\tilde{x}) \frac{\Delta}{D}\tilde{\partial}_\sigma \xi^\sigma(\tilde{x}) + \tilde{A}_\lambda(\tilde{x}) M_\nu{}^{\lambda}\right) - (\mu \leftrightarrow \nu)\\
    &=  \tilde{\partial}_\mu\left(\tilde{A}_\nu(\tilde{x})+\tilde{A}_\nu(\tilde{x}) \frac{\Delta}{D}\tilde{\partial}_\sigma \xi^\sigma(\tilde{x}) + \tilde{A}_\lambda(\tilde{x}) M_\nu{}^{\lambda}\right) + \tilde{\partial}_\mu \xi^{\lambda}(\tilde{x}) \tilde{\partial}_\lambda \tilde{A}_\nu(\tilde{x}) - (\mu \leftrightarrow \nu)\\
    &= \tilde{F}_{\mu\nu}(\tilde{x})+\tilde{F}_{\mu\nu}(\tilde{x}) \frac{\Delta}{D}\partial_\sigma \xi^\sigma(\tilde{x}) +   \tilde{A}_{(\nu}(\tilde{x}) \frac{\Delta}{D}\tilde{\partial}_{\mu)} \tilde{\partial}_\sigma \xi^\sigma(\tilde{x})   + \tilde{\partial}_{(\mu}(\tilde{A}_{\lambda}(\tilde{x})) M_{\nu)}{}^{\lambda} + \tilde{\partial}_{(\mu} \xi^{\lambda}(\tilde{x}) \tilde{\partial}_\lambda \tilde{A}_{\nu)}(\tilde{x})\\
  \end{align*}
  The contravariant equivalent of this result is given by 
  \begin{align*}
    F^{\mu \nu} = g^{\mu \sigma} g^{\nu \rho} F_{\sigma \rho} &= \Omega(\tilde{x})^{4}  \tilde{g}^{\mu \sigma} \tilde{g}^{\nu \rho} F_{\sigma \rho} \\
    &=\Omega(\tilde{x})^{4}  \left( \tilde{F}^{\mu\nu}(\tilde{x})+\tilde{F}^{\mu\nu}(\tilde{x}) \frac{\Delta}{D}\tilde{\partial}_\sigma \xi^\sigma(\tilde{x}) +  \tilde{g}^{\mu \sigma} \tilde{g}^{\nu \rho}    \tilde{A}_{(\nu}(\tilde{x}) \frac{\Delta}{D}\tilde{\partial}_{\mu)} \tilde{\partial}_\sigma \xi^\sigma(\tilde{x})   + \tilde{g}^{\mu \sigma} \tilde{g}^{\nu \rho} \tilde{\partial}_{(\sigma}(\tilde{A}_{\lambda}(\tilde{x})) M_{\rho)}{}^{\lambda}+ \tilde{g}^{\mu \sigma} \tilde{g}^{\nu \rho} \tilde{\partial}_{(\sigma} \xi^{\lambda}(\tilde{x}) \tilde{\partial}_\lambda \tilde{A}_{\rho)}(\tilde{x})  \right)
  \end{align*}
  
  Next, we calculate 
  \begin{align*}
    F_{\mu\nu} F^{\mu\nu} &= \left(\tilde{F}_{\mu\nu}(\tilde{x})+\tilde{F}_{\mu\nu}(\tilde{x}) \frac{\Delta}{D}\tilde{\partial}_\sigma \xi^\sigma(\tilde{x}) + \tilde{\partial}_{(\mu}(\tilde{A}_{\lambda}(\tilde{x})) M_{\nu)}{}^{\lambda} + \tilde{\partial}_{(\mu} \xi^{\lambda}(\tilde{x}) \tilde{\partial}_\lambda \tilde{A}_{\nu)}(\tilde{x}) + O(\xi^2)\right)\\
    &\times \Omega(\tilde{x})^{4}  \left( \tilde{F}^{\mu\nu}(\tilde{x})+\tilde{F}^{\mu\nu}(\tilde{x}) \frac{\Delta}{D}\tilde{\partial}_\sigma \xi^\sigma(\tilde{x}) +   \tilde{A}_{(\nu}(\tilde{x}) \frac{\Delta}{D}\tilde{\partial}_{\mu)} \tilde{\partial}_\sigma \xi^\sigma(\tilde{x}) + \tilde{g}^{\mu \sigma} \tilde{g}^{\nu \rho} \tilde{\partial}_{(\sigma}(\tilde{A}_{\lambda}(\tilde{x})) M_{\rho)}{}^{\lambda}+ \tilde{g}^{\mu \sigma} \tilde{g}^{\nu \rho} \tilde{\partial}_{(\sigma} \xi^{\lambda}(\tilde{x}) \tilde{\partial}_\lambda \tilde{A}_{\rho)}(\tilde{x})  \right)\\
    &= \Omega(\tilde{x})^4\left(\tilde{F}_{\mu\nu}(\tilde{x}) \tilde{F}^{\mu \nu}(\tilde{x}) + \tilde{F}_{\mu\nu}(\tilde{x})\tilde{F}^{\mu \nu}(\tilde{x}) \frac{2\Delta}{D} \tilde{\partial}_\sigma \xi^\sigma(\tilde{x}) + 2 \tilde{F}^{\mu\nu}\tilde{\partial}_{(\mu}(\tilde{A}_{\lambda}(\tilde{x}) ) M_{\nu)}{}^{\lambda}  + 2 \tilde{F}^{\mu\nu} \tilde{\partial}_{(\mu} \xi^{\lambda}(\tilde{x}) \tilde{\partial}_\lambda \tilde{A}_{\nu)}(\tilde{x}) +  2\tilde{F}^{\mu\nu}   \tilde{A}_{(\nu}(\tilde{x}) \frac{\Delta}{D}\tilde{\partial}_{\mu)} \tilde{\partial}_\sigma \xi^\sigma(\tilde{x})\right)\\
    &=  \Omega(\tilde{x})^4\left(\tilde{F}_{\mu\nu}(\tilde{x}) \tilde{F}^{\mu \nu}(\tilde{x}) + \tilde{F}_{\mu\nu}(\tilde{x})\tilde{F}^{\mu \nu}(\tilde{x}) \frac{2\Delta}{D} \tilde{\partial}_\sigma \xi^\sigma(\tilde{x}) + 2 \tilde{F}^{\mu\nu}\tilde{\partial}_{(\mu}(\tilde{A}_{\lambda}(\tilde{x}) ) M_{\nu)}{}^{\lambda}  + 2 \tilde{F}^{\mu\nu} \tilde{\partial}_{(\mu} \xi^{\lambda}(\tilde{x}) \tilde{\partial}_\lambda \tilde{A}_{\nu)}(\tilde{x}) +  4\tilde{F}^{\mu\nu} \tilde{A}_\nu(\tilde{x}) \frac{\Delta}{D}\tilde{\partial}_\mu \tilde{\partial}_\sigma \xi^\sigma(\tilde{x})\right)
  \end{align*}
  We want to show that the last line vanishes or is a total derivative.  
  
\end{enumerate}

\section{Axial anomaly}

\begin{enumerate}
  \item[(a)]
  \item[(b)] 
  \item[(c)]
  \item[(d)] 
\end{enumerate}

\section{OPE coefficients from three point functions}

\begin{enumerate}
  \item[(a)]
  \item[(b)] 
  \item[(c)]
  \item[(d)] 
\end{enumerate}


\section{Acknowledgement}


}

% References
\makereferences
%-------------------------------------------------------


%%%%%%%%%%%%%%%%%%%%%%%%
% Terminer le document %
%%%%%%%%%%%%%%%%%%%%%%%%
\end{document}
